wip

theories/SepROMode.v
@@ -590,6 +590,21 @@ Qed.*)
 
 Hint Rewrite heap_union_state : rew_fmap.
 
+Lemma heap_compat_components : forall h,
+  heap_compat h^rw h^ro.
+Admitted.
+
+Lemma heap_state_components : forall h,
+  heap_state h = heap_state (h^rw) \+ heap_state (h^ro).
+Proof using. 
+  intros. rewrite (heap_eq_union_rw_ro h) at 1.
+  rewrite* heap_union_state. applys* heap_compat_components.
+Qed.
+    
+  
+
+
+
 Hint Rewrite heap_union_empty_l heap_union_empty_r
   (* heap_full_f heap_full_r *)
   (*to_ro_f to_ro_r *) heap_union_f heap_union_r : rew_heap.
@@ -856,6 +871,18 @@ Class Normal (H:hprop) : Prop :=
 
 Hint Mode Normal ! : typeclass_instances.
 
+Lemma Normal_ro : forall H h,
+  Normal H ->
+  H h ->
+  h^ro = Fmap.empty.
+Proof using. introv N K. applys* N. Qed.
+
+Lemma Normal_rw : forall H h,
+  Normal H ->
+  H h ->
+  h^rw = h.
+Proof using. skip. Qed.
+
 Notation Normal_post Q := (forall x, Normal (Q x)).
 
 (* TEMP *)
@@ -1106,6 +1133,14 @@ Proof using.
   exists h' v. splits~. { himpl_fold. auto. }
 Qed.
 
+
+Lemma hoare_named_heap : forall t H Q,
+  (forall h, H h -> hoare t (= h) Q) ->
+  hoare t H Q.
+Proof using. introv M. intros h Hh. applys* M. Qed.
+
+
+
 Hint Rewrite to_ro_rw to_ro_ro : rew_heap.
 
 Lemma hoare_frame_read_only : forall t H1 Q1 H2,
@@ -1142,173 +1177,133 @@ Qed. (* TODO *)
 (** * Hoare rules for term constructs *)
 
 Implicit Types v : val.
-(*
-Lemma hoare_evalctx : forall C t1 H Q Q1,
-  evalctx C ->
-  hoare t1 H Q1 ->
-  (forall v, hoare (C v) (Q1 v) Q) ->
-  hoare (C t1) H Q.
-Proof using.
-  introv HC M1 M2 Hh.
-  forwards* (h1'&v1&R1&K1): (rm M1).
-  forwards* (h2'&v2&R2&K2): (rm M2).
-  exists h2' v2. splits~. { applys~ eval_evalctx R2. }
+
+
+Lemma hoare_hexists : forall t (A:Type) (J:A->hprop) Q,
+  (forall x, hoare t (J x) Q) ->
+  hoare t (hexists J) Q.
+Proof. introv M. intros h (x&Hh). applys M Hh. Qed.
+
+Lemma hoare_hpure : forall t (P:Prop) H Q,
+  (P -> hoare t H Q) ->
+  hoare t (\[P] \* H) Q.
+Proof.
+  introv M. intros h (h1&h2&(HP&M1)&M2&D&U). hnf in M1. subst. rew_heap*.
 Qed.
+
+
+(* ########################################################### *)
+(** ** Reasoning rules for terms, for Hoare triples. *)
 
 Lemma hoare_val : forall v H Q,
+  Normal_post Q ->
   H ==> Q v ->
   hoare (trm_val v) H Q.
-Proof using.
-  introv M. intros h Hh. exists h v. splits.
+Proof.
+  introv N M. intros h K. exists h v. splits~.
   { applys eval_val. }
-  { himpl_fold~. }
-Qed.
-
-Lemma hoare_fixs : forall f xs t1 H Q,
-  xs <> nil ->
-  H ==> Q (val_fixs f xs t1) ->
-  hoare (trm_fixs f xs t1) H Q.
-Proof using.
-  introv N M. intros h Hh. exists___. splits.
-  { applys~ eval_fixs. }
-  { himpl_fold~. }
+  { specializes M K. rewrites~ (>> Normal_rw M). }
 Qed.
 
 Lemma hoare_fix : forall f x t1 H Q,
+  Normal_post Q ->
   H ==> Q (val_fix f x t1) ->
   hoare (trm_fix f x t1) H Q.
-Proof using.
-  introv N M. intros h Hh. exists___. splits.
-  { applys~ eval_fixs. }
-  { himpl_fold~. }
+Proof.
+  introv N M. intros h K. exists h (val_fix f x t1). splits~.
+  { applys* eval_fix. }
+  { specializes M K. rewrites~ (>> Normal_rw M). }
 Qed.
 
-Proof using. introv M. applys hoare_fixs; auto_false. Qed.
-
-Lemma hoare_constr : forall id vs H Q,
-  H ==> Q (val_constr id vs) ->
-  hoare (trm_constr id (trms_vals vs)) H Q.
-Proof using.
-  introv M. intros h Hh. exists h (val_constr id vs). splits.
-  { applys eval_constr. }
-  { himpl_fold~. }
+Lemma hoare_app : forall v1 v2 (f:var) x t1 H Q,
+  Normal_post Q ->
+  v1 = val_fix f x t1 ->
+  f <> x ->
+  hoare (subst x v2 (subst f v1 t1)) H Q ->
+  hoare (trm_app v1 v2) H Q.
+Proof.
+  introv N E D M. intros s K0. forwards (s'&v&R1&K1&E1): (rm M) K0.
+  exists s' v. splits~. { applys* eval_app E R1. auto_false. }
 Qed.
 
-Lemma hoare_constr_trm : forall id ts t1 vs H Q Q1,
-  hoare t1 H Q1 ->
-  (forall v, hoare (trm_constr id ((trms_vals vs)++(trm_val v)::ts)) (Q1 v) Q) ->
-  hoare (trm_constr id ((trms_vals vs)++t1::ts)) H Q.
-Proof using.
-  introv M1 M2. intros h Hh.
-  forwards* (h1'&v1&R1&K1): (rm M1).
-  forwards* (h2'&v2&R2&K2): (rm M2).
-  exists h2' v2. splits~. { applys~ eval_constr_trm R2. }
-Qed.
+Hint Extern 1 (heap_compat _ _) => skip.
+Hint Extern 1 (disjoint _ _) => skip.
 
-Lemma hoare_let : forall z t1 t2 H Q Q1,
-  hoare t1 H Q1 ->
-  (forall v, hoare (subst1 z v t2) (Q1 v) Q) ->
-  hoare (trm_let z t1 t2) H Q.
-Proof using.
-  introv M1 M2 Hh.
-  forwards* (h1'&v1&R1&K1): (rm M1).
-  forwards* (h2'&v2&R2&K2): (rm M2).
-  exists h2' v2. splits~. { applys~ eval_let_trm R2. }
-Qed.
+Axiom RO_ro : forall h,
+  RO (= (h^ro)) (h^ro).
 
-Lemma hoare_seq : forall t1 t2 H Q H1,
-  hoare t1 H (fun r => H1) ->
-  hoare t2 H1 Q ->
-  hoare (trm_seq t1 t2) H Q.
-Proof using. introv M1 M2. applys* hoare_let. Qed.
+Axiom ro_ro : forall h,
+  (h^ro)^ro = h^ro.
+
+Axiom rw_ro : forall h,
+  (h^rw)^ro = Fmap.empty.
+
+Axiom ro_rw : forall h,
+  (h^ro)^rw = Fmap.empty.
+
+Hint Rewrite rw_ro ro_rw ro_ro heap_union_state to_ro_state : rew_heap.
+
+Lemma hoare_let : forall x t1 t2 H1 H2 Q Q1,
+  hoare t1 (H1 \* RO H2) Q1 ->
+  (forall v H3, hoare (subst x v t2) (Q1 v \* H2 \* RO H3) Q) ->
+  hoare (trm_let x t1 t2) (H1 \* H2) Q.
+Proof.
+  introv M1 M2 (h1&h2&P1&P2&D&U).
+  forwards* (h1'&v1&R1&K1&E1): (rm M1) (h1 \u to_ro h2).
+  { do 2 esplit. splits*. { applys* to_ro_pred. } }
+  forwards* (h2'&v2&R2&K2&E2): (rm M2) v1 (= (h1^ro)) (h1'^rw \u h2 \u h1^ro).
+  { do 2 esplit. (* TODO: tactic *) splits*.
+    do 2 esplit. splits*. applys RO_ro. } 
+  exists h2' v2. splits*.
+  { applys eval_let_trm (heap_state h1').
+    { applys_eq R1. subst h. rew_heap*. } 
+    { applys_eq R2. rewrite (heap_state_components h1').
+      rewrite E1. rew_heap*. fmap_eq*. } }
+    { rewrite E2. rewrite U. rew_heap*. }
+Qed.
 
 Lemma hoare_if : forall (b:bool) t1 t2 H Q,
   hoare (if b then t1 else t2) H Q ->
   hoare (trm_if b t1 t2) H Q.
-Proof using.
-  introv M1. intros h Hh. forwards* (h1'&v1&R1&K1): (rm M1).
-  exists h1' v1. splits~. { applys* eval_if. }
+Proof.
+  introv M1. intros h Hh. forwards* (h1'&v1&R1&K1&E1): (rm M1).
+  exists h1' v1. splits*. { applys* eval_if. }
 Qed.
-
-Lemma hoare_if_trm : forall Q1 t0 t1 t2 H Q,
-  hoare t0 H Q1 ->
-  (forall v, hoare (trm_if v t1 t2) (Q1 v) Q) ->
-  hoare (trm_if t0 t1 t2) H Q.
-Proof using.
-  introv M1 M2. applys* hoare_evalctx (fun t0 => trm_if t0 t1 t2).
-  { constructor. }
-Qed.
-
-Lemma hoare_apps_funs : forall xs F vs t1 H Q,
-  F = (val_funs xs t1) ->
-  var_funs xs (length vs) ->
-  hoare (substn xs vs t1) H Q ->
-  hoare (trm_apps F vs) H Q.
-Proof using.
-  introv E N M. intros h Hh. forwards* (h'&v&R&K): (rm M).
-  exists h' v. splits~. { subst. applys* eval_apps_funs. }
-Qed.
-
-Lemma hoare_apps_fixs : forall xs (f:var) F vs t1 H Q,
-  F = (val_fixs f xs t1) ->
-  var_fixs f xs (length vs) ->
-  hoare (substn (f::xs) (F::vs) t1) H Q ->
-  hoare (trm_apps F vs) H Q.
-Proof using.
-  introv E N M. intros h Hh. forwards* (h'&v&R&K): (rm M).
-  exists h' v. splits~. { subst. applys* eval_apps_fixs. }
-Qed.
-
-Lemma hoare_while_raw : forall t1 t2 H Q,
-  hoare (trm_if t1 (trm_seq t2 (trm_while t1 t2)) val_unit) H Q ->
-  hoare (trm_while t1 t2) H Q.
-Proof using.
-  introv M Hh. forwards* (h1'&v1&R1&K1): (rm M).
-  exists h1' v1. splits~. { applys* eval_while. }
-Qed.
-
-Lemma hoare_for_raw : forall (x:var) (n1 n2:int) t3 H Q,
-  hoare (
-    If (n1 <= n2)
-      then (trm_seq (subst1 x n1 t3) (trm_for x (n1+1) n2 t3))
-      else val_unit) H Q ->
-  hoare (trm_for x n1 n2 t3) H Q.
-Proof using.
-  introv M Hh. forwards* (h1'&v1&R1&K1): (rm M).
-  exists h1' v1. splits~. { applys* eval_for. }
-Qed.
-
-Lemma hoare_match : forall v p t1 pts H Q,
-  (forall (G:ctx), Ctx.dom G = patvars p -> v = patsubst G p -> hoare (isubst G t1) H Q) ->
-  ((forall (G:ctx), Ctx.dom G = patvars p -> v <> patsubst G p) -> hoare (trm_match v pts) H Q) ->
-  hoare (trm_match v ((p,t1)::pts)) H Q.
-Proof using.
-  introv M1 M2 Hh. tests C: (exists (G:ctx), Ctx.dom G = patvars p /\ v = patsubst G p).
-  { destruct C as (G&DG&Ev). forwards* (h1'&v1&R1&K1): (rm M1).
-    exists h1' v1. splits~. { applys~ eval_match_yes R1. } }
-  { forwards* (h1'&v1&R1&K1): (rm M2).
-    exists h1' v1. splits~. { applys~ eval_match_no R1.
-      intros G HG. specializes C G. rew_logic in C. destruct* C. } }
-Qed.
-
-Lemma hoare_case_trm : forall t1 pts H Q Q1,
-  hoare t1 H Q1 ->
-  (forall v, hoare (trm_match v pts) (Q1 v) Q) ->
-  hoare (trm_match t1 pts) H Q.
-Proof using.
-  introv M1 M2. intros h Hh.
-  forwards* (h1'&v1&R1&K1): (rm M1).
-  forwards* (h2'&v2&R2&K2): (rm M2).
-  exists h2' v2. splits~. { applys~ eval_match_trm R2. }
-Qed.
-*)
 
 
 (* ---------------------------------------------------------------------- *)
 (* ** Definition of SL triples in a logic with read-only predicates *)
 
 Definition triple (t:trm) (H:hprop) (Q:val->hprop) :=
-  forall H', Normal H' -> hoare t (H \* H') (Q \*+ H' (* \*+ \GC *)).
+  forall H', Normal H' -> hoare t (H \* H') (Q \*+ H' \*+ \GC).
+
+
+
+(* ---------------------------------------------------------------------- *)
+(* ** Connection with Hoare triples *)
+
+(** Lemma to introduce hoare instances for establishing triples,
+    integrating the consequence rule. *)
+
+Lemma triple_of_hoare : forall t H Q,
+  (forall H', exists Q', hoare t (H \* H') Q' /\ Q' ===> Q \*+ H' \*+ \GC) ->
+  triple t H Q.
+Proof using.
+  introv M. intros HF N. lets (Q'&R&W): M HF. applys* hoare_conseq R.
+Qed.
+
+(** Lemma to reciprocally deduce a hoare triple from a SL triple *)
+
+Lemma hoare_of_triple : forall t H Q HF,
+  triple t H Q ->
+  hoare t ((H \* HF) \* \GC) (fun r => (Q r \* HF) \* \GC).
+Proof using.
+  introv M. applys hoare_conseq. { applys M. } { xsimpl. } { xsimpl. }
+Qed.
+
+
+(* ---------------------------------------------------------------------- *)
+(* ** SL rules structural *)
 
 Lemma triple_frame_read_only : forall t H1 Q1 H2,
   triple t (H1 \* RO H2) Q1 ->
@@ -1323,6 +1318,272 @@ Proof using.
 Qed.
 
 
+Lemma triple_conseq : forall t H' Q' H Q,
+  triple t H' Q' ->
+  H ==> H' ->
+  Q' ===> Q ->
+  triple t H Q.
+Proof using. intros. applys* local_conseq. Qed.
+
+Lemma triple_frame : forall t H Q H',
+  triple t H Q ->
+  triple t (H \* H') (Q \*+ H').
+Proof using. intros. applys* local_frame. Qed.
+
+Lemma triple_ramified_frame : forall H1 Q1 t H Q,
+  triple t H1 Q1 ->
+  H ==> H1 \* (Q1 \--* Q) ->
+  triple t H Q.
+Proof using. intros. applys* local_ramified_frame. Qed.
+
+Lemma triple_ramified_frame_hgc : forall H1 Q1 t H Q,
+  triple t H1 Q1 ->
+  H ==> H1 \* (Q1 \--* (Q \*+ \GC)) ->
+  triple t H Q.
+Proof using. intros. applys* local_ramified_frame_hgc. Qed.
+
+Lemma triple_ramified_frame_htop : forall H1 Q1 t H Q,
+  triple t H1 Q1 ->
+  H ==> H1 \* (Q1 \--* (Q \*+ \Top)) ->
+  triple t H Q.
+Proof using. introv M1 W. rewrite <- hgc_eq_htop in W. applys* triple_ramified_frame_hgc. Qed.
+
+Lemma triple_hgc_pre : forall t H Q,
+  triple t H Q ->
+  triple t (H \* \GC) Q.
+Proof using. intros. applys* local_hgc_pre. Qed.
+
+Lemma triple_hgc_post : forall t H Q,
+  triple t H (Q \*+ \GC) ->
+  triple t H Q.
+Proof using. intros. applys* local_hgc_post. Qed.
+
+Lemma triple_htop_pre : forall t H Q,
+  triple t H Q ->
+  triple t (H \* \Top) Q.
+Proof using. introv M. rewrite <- hgc_eq_htop. applys* triple_hgc_pre. Qed.
+
+Lemma triple_htop_post : forall t H Q,
+  triple t H (Q \*+ \Top) ->
+  triple t H Q.
+Proof using. introv M. rewrite <- hgc_eq_htop in M. applys* triple_hgc_post. Qed.
+
+Lemma triple_hany_pre : forall t H H' Q,
+  triple t H Q ->
+  triple t (H \* H') Q.
+Proof using.
+  introv M. applys triple_conseq.
+  { applys* triple_htop_pre. }
+  { xsimpl. } { xsimpl. }
+Qed.
+
+Lemma triple_hany_post : forall t H H' Q,
+  triple t H (Q \*+ H') ->
+  triple t H Q.
+Proof using.
+  introv M. applys triple_htop_post.
+  applys triple_conseq M; xsimpl.
+Qed.
+
+Lemma triple_hexists : forall t (A:Type) (J:A->hprop) Q,
+  (forall x, triple t (J x) Q) ->
+  triple t (hexists J) Q.
+Proof using. intros. applys* local_hexists. Qed.
+
+Lemma triple_hforall : forall A (x:A) t (J:A->hprop) Q,
+  triple t (J x) Q ->
+  triple t (hforall J) Q.
+Proof using. intros. applys* local_hforall. Qed.
+
+Lemma triple_hpure : forall t (P:Prop) H Q,
+  (P -> triple t H Q) ->
+  triple t (\[P] \* H) Q.
+Proof using. intros. applys* local_hpure. Qed.
+
+Lemma triple_hwand_hpure_l : forall t (P:Prop) H Q,
+  P ->
+  triple t H Q ->
+  triple t (\[P] \-* H) Q.
+Proof using. intros. applys* local_hwand_hpure_l. Qed.
+
+Lemma triple_hor : forall t H1 H2 Q,
+  triple t H1 Q ->
+  triple t H2 Q ->
+  triple t (hor H1 H2) Q.
+Proof using. intros. applys* local_hor. Qed.
+
+Lemma triple_hand_l : forall t H1 H2 Q,
+  triple t H1 Q ->
+  triple t (hand H1 H2) Q.
+Proof using. intros. applys* local_hand_l. Qed.
+
+Lemma triple_hand_r : forall t H1 H2 Q,
+  triple t H2 Q ->
+  triple t (hand H1 H2) Q.
+Proof using. intros. applys* local_hand_r. Qed.
+
+Lemma triple_conseq_frame : forall H2 H1 Q1 t H Q,
+  triple t H1 Q1 ->
+  H ==> H1 \* H2 ->
+  Q1 \*+ H2 ===> Q ->
+  triple t H Q.
+Proof using. intros. applys* local_conseq_frame. Qed.
+
+Lemma triple_conseq_frame_hgc : forall H2 H1 Q1 t H Q,
+  triple t H1 Q1 ->
+  H ==> H1 \* H2 ->
+  Q1 \*+ H2 ===> Q \*+ \GC ->
+  triple t H Q.
+Proof using. intros. applys* local_conseq_frame_hgc. Qed.
+
+
+
+(* ---------------------------------------------------------------------- *)
+(* ** SL rules for terms *)
+
+Lemma triple_val : forall v H Q,
+  H ==> Q v ->
+  triple (trm_val v) H Q.
+Proof using.
+  introv M. intros HF. applys hoare_val. { xchanges M. }
+Qed.
+
+Lemma triple_fixs : forall f xs t1 H Q,
+  xs <> nil ->
+  H ==> Q (val_fixs f xs t1) ->
+  triple (trm_fixs f xs t1) H Q.
+Proof using.
+  introv N M. intros HF. applys~ hoare_fixs. { xchanges M. }
+Qed.
+
+Lemma triple_constr : forall id vs H Q,
+  H ==> Q (val_constr id vs) ->
+  triple (trm_constr id vs) H Q.
+Proof using.
+  introv M. intros HF. applys hoare_constr. { xchanges M. }
+Qed.
+
+Lemma triple_constr_trm : forall id ts t1 vs H Q Q1,
+  triple t1 H Q1 ->
+  (forall (X:val), triple (trm_constr id ((trms_vals vs)++(trm_val X)::ts)) (Q1 X) Q) ->
+  triple (trm_constr id ((trms_vals vs)++t1::ts)) H Q.
+Proof using.
+  introv M1 M2. intros HF. applys~ hoare_constr_trm.
+  { intros v. applys* hoare_of_triple. }
+Qed.
+
+Lemma triple_let : forall z t1 t2 H Q Q1,
+  triple t1 H Q1 ->
+  (forall (X:val), triple (subst1 z X t2) (Q1 X) Q) ->
+  triple (trm_let z t1 t2) H Q.
+Proof using.
+  introv M1 M2. intros HF. applys hoare_let.
+  { applys M1. }
+  { intros v. applys* hoare_of_triple. }
+Qed.
+
+Lemma triple_seq : forall t1 t2 H Q Q1,
+  triple t1 H Q1 ->
+  (forall (X:val), triple t2 (Q1 X) Q) ->
+  triple (trm_seq t1 t2) H Q.
+Proof using.
+  introv M1 M2. applys* triple_let. (* BIND intros. rewrite* subst1_anon. *)
+Qed.
+
+Lemma triple_if : forall (b:bool) t1 t2 H Q,
+  triple (if b then t1 else t2) H Q ->
+  triple (trm_if b t1 t2) H Q.
+Proof using.
+  introv M1. intros HF. applys hoare_if. applys M1.
+Qed.
+
+Lemma triple_if_bool : forall (b:bool) t1 t2 H Q,
+  (b = true -> triple t1 H Q) ->
+  (b = false -> triple t2 H Q) ->
+  triple (trm_if b t1 t2) H Q.
+Proof using.
+  introv M1 M2. applys triple_if. case_if*.
+Qed.
+
+Lemma triple_if_trm : forall Q1 t0 t1 t2 H Q,
+  triple t0 H Q1 ->
+  (forall v, triple (trm_if v t1 t2) (Q1 v) Q) ->
+  triple (trm_if t0 t1 t2) H Q.
+Proof using.
+  introv M1 M2. intros HF. applys* hoare_if_trm.
+  { intros v. applys* hoare_of_triple. }
+Qed.
+
+Lemma triple_if_trm' : forall Q1 t0 t1 t2 H Q, (* not very useful *)
+  triple t0 H Q1 ->
+  (forall (b:bool), triple (if b then t1 else t2) (Q1 b) Q) ->
+  (forall v, ~ is_val_bool v -> (Q1 v) ==> \[False]) ->
+  triple (trm_if t0 t1 t2) H Q.
+Proof using.
+  introv M1 M2 M3. applys* triple_if_trm.
+  { intros v. tests C: (is_val_bool v).
+    { destruct C as (b&E). subst. applys* triple_if. }
+    { xtchange* M3. xtpull ;=>. false. } }
+Qed.
+
+Lemma triple_apps_funs : forall xs F (Vs:vals) t1 H Q,
+  F = (val_funs xs t1) ->
+  var_funs xs (length Vs) ->
+  triple (substn xs Vs t1) H Q ->
+  triple (trm_apps F Vs) H Q.
+Proof using. introv E N M. intros HF. applys* hoare_apps_funs. Qed.
+
+Lemma triple_apps_fixs : forall xs (f:var) F (Vs:vals) t1 H Q,
+  F = (val_fixs f xs t1) ->
+  var_fixs f xs (length Vs) ->
+  triple (substn (f::xs) (F::Vs) t1) H Q ->
+  triple (trm_apps F Vs) H Q.
+Proof using. introv E N M. intros HF. applys* hoare_apps_fixs. Qed.
+
+(* ---------------------------------------------------------------------- *)
+(* ** SL rules for primitive functions over the state *)
+
+Lemma triple_ref : forall v,
+  triple (val_ref v)
+    \[]
+    (fun r => \exists l, \[r = val_loc l] \* l ~~~> v).
+Proof using.
+  intros. applys triple_of_hoare. intros HF. rew_heap.
+  esplit; split. { applys hoare_ref. } { xsimpl*. }
+Qed.
+
+Lemma triple_get : forall v l,
+  triple (val_get (val_loc l))
+    (l ~~~> v)
+    (fun x => \[x = v] \* (l ~~~> v)).
+Proof using.
+  intros. applys triple_of_hoare. intros HF.
+  esplit; split. { applys hoare_get. } { xsimpl*. }
+Qed.
+
+Lemma triple_set : forall w l v,
+  triple (val_set (val_loc l) w)
+    (l ~~~> v)
+    (fun r => \[r = val_unit] \* l ~~~> w).
+Proof using.
+  intros. applys triple_of_hoare. intros HF.
+  esplit; split. { applys hoare_set. } { xsimpl*. }
+Qed.
+
+Lemma triple_set' : forall w l v,
+  triple (val_set (val_loc l) w)
+    (l ~~~> v)
+    (fun r => l ~~~> w).
+Proof using. intros. xapplys* triple_set. Qed.
+
+Lemma triple_free : forall l v,
+  triple (val_free (val_loc l))
+    (l ~~~> v)
+    (fun r => \[r = val_unit]).
+Proof using.
+  intros. applys triple_of_hoare. intros HF.
+  esplit; split. { applys hoare_free. } { xsimpl*. }
+Qed.
 
 
 (* ********************************************************************** *)
